Program-proofs/Exercises/2D-counting/prob03/sol03Annotated.dfy
@@ -1,67 +1,63 @@
-/* file: sol03Annotated.dfy
-   author: David De Potter
-   description: extra practice in Dafny, 2D counting, 
-   solution to prob03, with annotations
-   This is exercise 9.4 from the PC reader
+/*  file: sol03Annotated.dfy
+    author: David De Potter
+    description: extra practice in Dafny, 2D counting, 
+    solution to prob03, with annotations
+    This is exercise 9.4 from the PC reader
 
-   NOTE: here we take the same approach as in prob02, by starting the search
-   from the upper-right corner and shrinking the rectangle in a south-western
-   direction by either decrementing x or y. 
+    NOTE: here we take the same approach as in prob02, by starting the 
+    search from the upper-right corner and shrinking the rectangle in 
+    a south-western direction by either decrementing x or y. 
 */
 
-ghost predicate DecrAsc(f:(int,int) -> int) 
-{
-    // Expresses the property that f is decreasing in its first 
-    // argument and ascending in its second argument, i.e. 
-    // ∀ i,j,k ∈ ℤ:
-    //   if i < j then f(i,k) > f(j,k)
-    //   if j ≤ k then f(i,j) ≤ f(i,k)
-  (forall i,j,k:: i <  j  ==>  f(i,k) >  f(j,k)) &&
-  (forall i,j,k:: j <= k  ==>  f(i,j) <= f(i,k))
-}
-
-function ord(b:bool): int
-{
-  if b then 1 else 0
-}
+include "../../commonSupport.dfy"
+import opened CommonFunctions
+import opened MonotonicityProps
 
 ghost function F(h:(int,int) -> int, x:int, y:int, w:int): int
-requires DecrAsc(h)
+requires Ordered2DInt(h, Decr, Asc)
 {   
     // We want to find a recursive definition of F that we can use to derive T.
     // F is defined as:
     //   F(h,x,y,w) = #{ (i,j) | i,j: 0 ≤ i < x ∧ 0 ≤ j < y ∧ h(i,j) = w }
-    // This function counts the number of points in the rectangle [0,x) × [0,y) 
-    // that satisfy h(i,j) = w. 
-    // Base case: x ≤ 0 or y ≤ 0, then the rectangle is empty and F(x,y) = # ∅ = 0.
-    // Recursive case: in this case we want to shrink the rectangle by either
-    //                 decrementing x or y. 
+    // This function counts the number of points in the rectangle 
+    // [0,x) × [0,y) that satisfy h(i,j) = w. 
+    //
+    // Base case: x ≤ 0 or y ≤ 0, then the rectangle is empty 
+    //            and F(x,y) = # ∅ = 0.
+    // Recursive case: here we want to shrink the rectangle by either
+    //                 - decrementing x (which removes the rightmost column)
+    //                 - decrementing y (which removes the topmost row)
     //
     // What happens if we decrement x? 
     //   F(x,y)
     //   = #{ (i,j) | i,j: 0 ≤ i < x ∧ 0 ≤ j < y ∧ h(i,j) = w }
-    //       ( split domain into 0 ≤ i < x-1 and i = x-1 )
+    //       ( split domain into 0 ≤ i < x-1 and the rightmost column i = x-1 )
     //   = #{ (i,j) | i,j: 0 ≤ i < x-1 ∧ 0 ≤ j < y ∧ h(i,j) = w }
     //     + #{ (x-1,j) | j: 0 ≤ j < y ∧ h(x-1,j) = w }
     //       ( apply definition of F to the first term )
     //   = F(h, x-1,y,w) + #{ (x-1,j) | j: 0 ≤ j < y ∧ h(x-1,j) = w }
-    //       ( h(x-1, j) is ascending in j, so the value of h(x-1,y-1) is maximal,
-    //         so if we assume h(x-1,y-1) < w, then h(x-1,j) < w for all 0 ≤ j < y )
+    //       ( h(x-1, j) is ascending in j, so the value of h(x-1,y-1) 
+    //         is maximal. If we assume h(x-1,y-1) < w, then h(x-1,j) < w 
+    //         for all 0 ≤ j < y and we can discard the whole column x-1 
+    //         as it contains no matching points )
     //   = F(h, x - 1,y,w) + # ∅
     //   = F(h, x - 1,y,w)
     //
     // What happens if we decrement y?
     //   F(h,x,y,w)
     //   = #{ (i,j) | i,j: 0 ≤ i < x ∧ 0 ≤ j < y ∧ h(i,j) = w }
-    //       ( split domain into 0 ≤ j < y-1 and j = y-1 )
+    //       ( split domain into 0 ≤ j < y-1 and the topmost row j = y-1 )
     //   = #{ (i,j) | i,j: 0 ≤ i < x ∧ 0 ≤ j < y-1 ∧ h(i,j) = w }
     //     + #{ (i,y-1) | i: 0 ≤ i < x ∧ h(i,y-1) = w }
     //       ( apply definition of F to the first term )
     //   = F(h, x, y-1, w) + #{ (i,y-1) | i: 0 ≤ i < x ∧ h(i,y-1) = w }
-    //       ( h(i,y-1) is strictly decreasing in i, so the value of h(x-1,y-1) is  
-    //         minimal, so if we assume h(x-1,y-1) ≥ w, then either h(x-1,y-1) = w 
-    //         for only that point or h(i,y-1) > w for all 0 ≤ i < x )
-    //   = F(h, x, y-1, w) + ord(h(x-1,y-1) = w) 
+    //       ( h(i,y-1) is strictly decreasing in i, so the value of 
+    //         h(x-1,y-1) is minimal. If we assume h(x-1,y-1) ≥ w, then 
+    //         either h(x-1,y-1) = w for only that point or h(i,y-1) > w 
+    //         for all 0 ≤ i < x. So we add one matching point to the 
+    //         overall count if h(x-1,y-1) = w, after which we can discard 
+    //         the whole row y-1 )
+    //   = F(h, x, y-1, w) + ord(h(x-1,y-1) = w)
 
   if x <= 0 || y <= 0 then 0
   else if h(x - 1, y - 1) < w then F(h, x - 1, y, w)
@@ -70,7 +66,7 @@ requires DecrAsc(h)
 
 method problem03(h:(int,int) -> int, m:nat, n:nat, w:int) 
 returns (z: int)
-requires DecrAsc(h)
+requires Ordered2DInt(h, Decr, Asc)
 ensures z == F(h, m ,n, w)
 {
     // Initialization to establish J before the loop
@@ -87,14 +83,15 @@ ensures z == F(h, m ,n, w)
   {
       // J ∧ B ∧ vf = V
       // z + F(h,x,y,w) = Z ∧ x > 0 ∧ y > 0 ∧ x + y = V
-      //   ( we want to apply the recursive definition of F, so we need 
-      //     to distinguish the cases h(x-1,y-1) < w and h(x-1,y-1) ≥ w )
+      //   ( to apply the recursive definition of F, we need to
+      //     distinguish the cases h(x-1,y-1) < w and h(x-1,y-1) ≥ w )
 
     if h(x - 1, y - 1) < w
     {
-        // z + F(h,x,y,w) = Z ∧ h(x-1,y-1) < w ∧ x > 0 ∧ y > 0 ∧ x + y = V
-        //   ( apply definition of F; 
-        //     since x > 0 ∧ y > 0, we are not in the base case )
+        // z + F(h,x,y,w) = Z ∧ h(x-1,y-1) < w ∧ x > 0 ∧ y > 0 
+        //   ∧ x + y = V
+        //   ( apply definition of F; since x > 0 ∧ y > 0, 
+        //     we are not in the base case )
         // z + F(h,x-1,y,w) = Z ∧ x + y = V
         //   ( prepare for decrementing x )
         // z + F(h,x-1,y,w) = Z ∧ x - 1 + y < V
@@ -104,9 +101,10 @@ ensures z == F(h, m ,n, w)
 
     else
     {
-        // z + F(h,x,y,w) = Z ∧ h(x-1,y-1) ≥ w ∧ x > 0 ∧ y > 0 ∧ x + y = V
-        //   ( apply definition of F; 
-        //     since x > 0 ∧ y > 0, we are not in the base case )
+        // z + F(h,x,y,w) = Z ∧ h(x-1,y-1) ≥ w ∧ x > 0 ∧ y > 0 
+        //   ∧ x + y = V
+        //   ( apply definition of F; since x > 0 ∧ y > 0, 
+        //     we are not in the base case )
         // z + F(h,x,y-1,w) + ord(h(x-1,y-1) = w) = Z ∧ x + y = V
       z := z + ord(h(x - 1, y - 1) == w);
         // z + F(h,x,y-1,w) = Z ∧ x + y = V
